src/simple-proof/alg-proof/Concepts.v
@@ -1,0 +1,20 @@
+Require Import Metalib.Metatheory.
+
+
+Class CanOpen (A : Type) :=
+  {
+    open_rec (k : nat) (u : var) (ins : A) : A
+  }.
+Hint Unfold open_rec.
+
+Class HasFv (A : Type) :=
+  {
+    fv (ins : A) : atoms
+  }.
+Hint Unfold fv.
+
+Class CanSubst (A : Type) :=
+  {
+    substi (z u : var) (ins : A) : A
+  }.
+Hint Unfold substi.
