src/simple-proof/alg-proof/Substitution.v
@@ -1,0 +1,140 @@
+Set Implicit Arguments.
+
+Require Import Definitions.
+Require Import LibUtils.
+Require Import Coq.Lists.List.
+Require Import Concepts.
+Require Import Metalib.Metatheory.
+
+Section SubstDefinitions.
+
+  Variable z u : var.
+
+  Definition subst_avar (a : avar) : avar :=
+    match a with
+    | avar_b i as a => a
+    | avar_f x => avar_f $ if x == z then u else x
+    end.
+
+  Fixpoint subst_typ (T : typ) : typ :=
+    match T with
+    | typ_top => ⊤
+    | typ_bot => ⊥
+    | typ_sel x L => (subst_avar x) ⋅ L
+    | typ_all T U => all( subst_typ T ) subst_typ U
+    | typ_obj DS => μ{ subst_decs DS }
+    end
+  with
+  subst_dec (D : dec) : dec :=
+    match D with
+    | dec_typ T U => dec_typ (subst_typ T) $ subst_typ U
+    | dec_trm T => dec_trm $ subst_typ T
+    end
+  with
+  subst_decs (DS : decs) : decs :=
+    match DS with
+    | decs_nil => decs_nil
+    | decs_cons L D DS' => decs_cons L (subst_dec D) $ subst_decs DS'
+    end.
+
+  Fixpoint subst_trm (t : trm) : trm :=
+    match t with
+    | trm_var x => trm_var $ subst_avar x
+    | trm_val v => trm_val $ subst_val v
+    | trm_sel x L => trm_sel (subst_avar x) L
+    | trm_app x1 x2 => trm_app (subst_avar x1) $ subst_avar x2
+    | trm_let t1 t2 => trm_let (subst_trm t1) $ subst_trm t2
+    end
+  with
+  subst_val (v : val) : val :=
+    match v with
+    | ν( DS ){ ds } => ν( subst_decs DS ){ subst_defs ds }
+    | λ( T ){ t } => λ( subst_typ T ){ subst_trm t }
+    end
+  with
+  subst_def (d : def) : def :=
+    match d with
+    | def_typ T => def_typ $ subst_typ T
+    | def_trm t => def_trm $ subst_trm t
+    end
+  with
+  subst_defs (ds : defs) : defs :=
+    match ds with
+    | defs_nil => defs_nil
+    | defs_cons L d ds' => defs_cons L (subst_def d) $ subst_defs ds'
+    end.
+
+End SubstDefinitions.
+
+Instance SubstAvar : CanSubst avar := { substi := subst_avar }.
+Instance SubstTyp : CanSubst typ := { substi := subst_typ }.
+Instance SubstDec : CanSubst dec := { substi := subst_dec }.
+Instance SubstDecs : CanSubst decs := { substi := subst_decs }.
+Instance SubstTrm : CanSubst trm := { substi := subst_trm }.
+Instance SubstVal : CanSubst val := { substi := subst_val }.
+Instance SubstDef : CanSubst def := { substi := subst_def }.
+Instance SubstDefs : CanSubst defs := { substi := subst_defs }.
+
+Section OpenFreshInj.
+  Variable z : atom.
+
+  Local Notation fresh_inj T :=
+    (forall (x y : T) k,
+      z `notin` fv x ->
+      z `notin` fv y ->
+      open_rec k z x = open_rec k z y ->
+      x = y).
+  
+  Lemma open_fresh_inj_avar : fresh_inj avar.
+  Proof.
+    intros. destruct x, y; routine.
+  Qed.
+
+  Local Hint Resolve open_fresh_inj_avar.
+
+  Local Ltac boom :=
+    mutual induction;
+    routine_impl ltac:(idtac;
+    match goal with
+    | [ H : _ = _ _ z ?t' |- _ ] =>
+      destruct t'; repeat f_equal; inversion H
+    end);
+    simpl in *; eauto with alg_def.
+  
+  Lemma open_fresh_inj_typ_dec_decs :
+    fresh_inj typ /\ fresh_inj dec /\ fresh_inj decs.
+  Proof. boom. Qed.
+
+  Hint Extern 1 => eapp_conj open_fresh_inj_typ_dec_decs.
+  
+  Lemma open_fresh_inj_trm_val_def_defs :
+    fresh_inj trm /\ fresh_inj val /\ fresh_inj def /\ fresh_inj defs.
+  Proof. boom. Qed.
+  
+End OpenFreshInj.
+
+
+Section SubstFresh.
+  Variable x y : var.
+
+  Local Notation subst_fresh T :=
+    (forall t : T, x `notin` fv t -> substi x y t = t).
+
+  Lemma subst_fresh_avar : subst_fresh avar.
+  Proof.
+    intros. destruct t; routine.
+  Qed.
+
+  Local Hint Resolve subst_fresh_avar.
+
+  Lemma subst_fresh_typ_dec_decs :
+    subst_fresh typ /\ subst_fresh dec /\ subst_fresh decs.
+  Proof. mutual induction; routine. Qed.
+
+  Local Hint Extern 1 => eapp_conj subst_fresh_typ_dec_decs.
+
+  Lemma subst_fresh_trm_val_def_defs :
+    subst_fresh trm /\ subst_fresh val /\ subst_fresh def /\ subst_fresh defs.
+  Proof. mutual induction; routine. Qed.
+  
+End SubstFresh.
