src/simple-proof/alg-proof/SyntacticProperties.v
@@ -1,0 +1,26 @@
+
+Set Implicit Arguments.
+
+Require Import Definitions.
+Require Import LibUtils.
+Require Import Coq.Lists.List.
+
+Section ObjectProps.
+
+  Lemma obj_exchg_equiv : forall G (DS1 DS2 : decs),
+      not_empty DS1 ->
+      not_empty DS2 ->
+      G ⊢ μ{ append DS1 DS2 } ≊ μ{ append DS2 DS1 }.
+  Proof. 
+    intros; split; intros;
+      constructor; auto with alg_def;
+      autounfold;
+      rewrite append_sound;
+      match goal with
+      | [  |- context[?DS1 ++ ?DS2] ] =>
+        replace (DS1 ++ DS2) with (nil ++ DS1 ++ DS2) by trivial
+      end;
+      eapply not_empty_relax; trivial.
+  Qed.
+
+End ObjectProps.
